Prove the existence of promise steps

src/AtoP.v
@@ -29,7 +29,7 @@ Lemma linearize A
     <<PERM: Permutation l l'>> /\
     <<REL: forall i j x y
              (X: List.nth_error l' i = Some x)
-             (X: List.nth_error l' j = Some y)
+             (Y: List.nth_error l' j = Some y)
              (REL: rel x y),
         i < j>>.
 Proof.
@@ -53,6 +53,17 @@ Fixpoint filter_map A B (f: A -> option B) (l: list A): list B :=
     end
   end.
 
+Lemma in_filter_map_iff A B (f: A -> option B) (l: list A) (b: B):
+  List.In b (filter_map f l) <-> exists a, List.In a l /\ f a = Some b.
+Proof.
+  induction l; ss.
+  { econs; i; des; ss. }
+  destruct (f a) eqn:FA; ss.
+  - rewrite IHl. intuition; des; subst; eauto.
+    rewrite FA in H2. inv H2. auto.
+  - rewrite IHl. intuition; des; subst; eauto. congr.
+ Qed.
+
 Definition mem_of_ex
            (ex:Execution.t)
            (eids:list eidT):
@@ -65,9 +76,78 @@ Definition mem_of_ex
        end)
     eids.
 
+Definition list_rev_list_rect
+           (A:Type)
+           (P:list A -> Type)
+           (INIT: P [])
+	         (STEP: forall (a:A) (l:list A), P (List.rev l) -> P (List.rev (a :: l))):
+	forall l:list A, P (List.rev l).
+Proof.
+  induction l; auto.
+Defined.
+
+Definition list_rev_rect
+           (A:Type)
+           (P:list A -> Type)
+           (INIT: P [])
+           (STEP: forall x l, P l -> P (l ++ [x])):
+  forall l, P l.
+Proof.
+  intros.
+  generalize (List.rev_involutive l).
+  intros E; rewrite <- E.
+  apply (list_rev_list_rect P).
+  auto.
+
+  simpl.
+  intros.
+  apply (STEP a (List.rev l0)).
+  auto.
+Defined.
+
 Definition promises_from_mem
-           (tid: Id.t) (mem: Memory.t): Promises.t :=
-  Promises.empty. (* TODO *)
+           (tid: Id.t) (mem: Memory.t): Promises.t.
+Proof.
+  induction mem using list_rev_rect.
+  - apply Promises.empty.
+  - destruct x.
+    apply (if tid0 == tid
+           then Promises.set (S (List.length (List.rev mem))) IHmem
+           else IHmem).
+Defined.
+
+Lemma promises_from_mem_empty tid:
+  promises_from_mem tid Memory.empty = Promises.empty.
+Proof.
+  unfold promises_from_mem, list_rev_rect, eq_rect. ss.
+  match goal with
+  | [|- context[match ?c with | eq_refl => _ end]] => destruct c
+  end; ss.
+Qed.
+
+Lemma promises_from_mem_snoc tid mem msg:
+  promises_from_mem tid (mem ++ [msg]) =
+  if msg.(Msg.tid) == tid
+  then Promises.set (S (List.length mem)) (promises_from_mem tid mem)
+  else promises_from_mem tid mem.
+Proof.
+  unfold promises_from_mem at 1, list_rev_rect, eq_rect.
+  match goal with
+  | [|- context[match ?c with | eq_refl => _ end]] => destruct c
+  end; ss.
+  rewrite List.rev_involutive, List.rev_app_distr. ss.
+  destruct msg. s. condtac.
+  - inversion e. subst. rewrite ? List.rev_length.
+    f_equal.
+    unfold promises_from_mem, list_rev_rect, eq_rect.
+    match goal with
+    | [|- context[match ?c with | eq_refl => _ end]] => destruct c
+    end; ss.
+  - unfold promises_from_mem, list_rev_rect, eq_rect.
+    match goal with
+    | [|- context[match ?c with | eq_refl => _ end]] => destruct c
+    end; ss.
+Qed.
 
 Definition Local_init_with_promises
            (promises: Promises.t): Local.t :=
@@ -97,7 +177,11 @@ Lemma promise_mem
     <<MEM: m.(Machine.mem) = mem>>.
 Proof.
   revert MEM. induction mem using List.rev_ind; i.
-  { esplits; eauto. apply IdMap.map_spec. }
+  { esplits; eauto. i. s. rewrite IdMap.map_spec.
+    destruct (IdMap.find tid p); ss.
+    unfold Local.init, Local_init_with_promises. repeat f_equal.
+    rewrite promises_from_mem_empty. ss.
+  }
   exploit IHmem; eauto.
   { i. apply MEM. apply List.in_app_iff. intuition. }
   i. des. subst. destruct x.
@@ -116,10 +200,12 @@ Proof.
   - s. i. rewrite IdMap.add_spec. condtac; ss.
     + inversion e. subst. rewrite FIND. s.
       unfold Local_init_with_promises. repeat f_equal.
-      admit.
-    + rewrite TPOOL. ss.
+      rewrite promises_from_mem_snoc. condtac; ss.
+    + rewrite TPOOL. destruct (IdMap.find tid0 p); ss.
+      unfold Local_init_with_promises. rewrite promises_from_mem_snoc. s.
+      condtac; ss. congr.
   - ss.
-Admitted.
+Qed.
 
 Lemma axiomatic_to_promising
       p ex
@@ -136,8 +222,15 @@ Proof.
 
   (* Construct promise steps. *)
   exploit (promise_mem p mem); eauto.
-  { i. subst. admit. }
-  i. des.
+  { i. subst. unfold mem_of_ex in MSG. rewrite in_filter_map_iff in MSG. des.
+    symmetry in PERM. exploit Permutation_in; eauto. intro X.
+    generalize (Execution.eids_spec ex). i. des.
+    apply LABEL in X. destruct (Execution.label a ex) eqn:Y; ss.
+    destruct t; ss. inv MSG0. s. unfold Execution.label in Y.
+    inv AXIOMATIC. inv PRE. rewrite LABELS, IdMap.map_spec in Y.
+    destruct (IdMap.find (fst a) locals) eqn:Z; ss.
+    specialize (LOCALS (fst a)). inv LOCALS; ss. congr.
+  }
 
   (* TODO: execute each thread. *)
   admit.
